map

Spacetalk/Compiler.lean
@@ -48,7 +48,9 @@ structure SDFOneInputOneOutput (α β : Step.Prim) where
   one_output : g.fifos.filter FIFO.isOutput = [.output outFifo]
   out_ty_eq : outFifo.t = β.toSDF
   nodes_len : 0 < g.numNodes
+  out_producer : outFifo.producer = ⟨0, nodes_len⟩
   consumerPort : Member α.toSDF (g.nodes.get ⟨0, nodes_len⟩).inputs
+  output_eq : g.outputs = [β.toSDF]
 
 @[reducible]
 def Step.Ty.toSDF (sty : Step.Ty) :=
@@ -79,10 +81,12 @@ def binOpConstRightGraph {α β γ : Step.Prim} (op : SimpleDataflow.BinaryOp α
     by simp [fifos],
     by simp,
     outFifo,
-    by simp [fifos],
+    by simp [fifos, FIFO.isOutput],
     by simp,
     by simp,
-    .head
+    rfl,
+    .head,
+    rfl
   ⟩
 
 def Step.UnaryOp.compile : Step.UnaryOp α β → SDFOneInputOneOutput α β
@@ -93,28 +97,39 @@ def Step.BinaryOp.compile : Step.BinaryOp α β γ → SimpleDataflow.Ops [α.to
   | .add => .binaryOp .add
   | .mul => .binaryOp .mul
 
-class IndexConverter {α : Type u} {n m : Nat} (h_m : 0 < m) (xs : Vector α n) (ys : Vector α m) :=
+class IndexConverter {α : Type u} {n m : Nat} (xs : Vector α n) (ys : Vector α m) :=
   conv : Fin n → Fin m
   conv_congr : ∀ {i}, xs.get i = ys.get (conv i)
   conv_lt : ∀ ⦃i j⦄, i < j → conv i < conv j
-  conv_gt_zero: ∀ {i}, ⟨0, h_m⟩ < conv i
 
-def consConverter : IndexConverter (Nat.zero_lt_succ _) xs (x ::ᵥ xs.append ys) :=
+class IndexConverterGtZero {α : Type u} {n m : Nat} (xs : Vector α n) (ys : Vector α m) extends IndexConverter xs ys :=
+  conv_gt_zero: ∀ {i}, (h_m : 0 < m) → ⟨0, h_m⟩ < conv i
+
+def appendIdConverter : IndexConverter xs (xs.append ys) :=
+  let conv : Fin xs.length → Fin (xs.append ys).length := λ i ↦ ⟨i.val, by have := i.isLt; linarith⟩
+  have conv_congr : ∀ {i}, xs.get i = (xs.append ys).get (conv i) := by
+    intro i
+    simp [conv]
+    apply Vector.get_append_left.symm
+  have conv_lt : ∀ ⦃i j⦄, i < j → conv i < conv j := by intro i j; simp [conv]
+  ⟨conv, conv_congr, conv_lt⟩
+
+def consConverter : IndexConverterGtZero xs (x ::ᵥ xs.append ys) :=
   let conv : Fin xs.length → Fin (x ::ᵥ xs.append ys).length := λ i ↦ ⟨i.val + 1, by have := i.isLt; linarith⟩
   have conv_congr : ∀ {i}, xs.get i = (x ::ᵥ xs.append ys).get (conv i) := by
     intro i
     rw [←(x ::ᵥ xs.append ys).get_tail ⟨i, Nat.lt_add_right _ i.isLt⟩]
     exact Vector.get_append_left.symm
   have conv_lt : ∀ ⦃i j⦄, i < j → conv i < conv j := by simp [conv]
-  have conv_gt_zero: ∀ {i}, 0 < conv i := by
+  have conv_gt_zero: ∀ {i}, _ → 0 < conv i := by
     intro i
     simp [conv]
     apply Fin.mk_lt_mk.mpr
     rw [Nat.zero_mod]
     simp
-  ⟨conv, conv_congr, conv_lt, conv_gt_zero⟩
+  .mk conv_gt_zero (toIndexConverter := ⟨conv, conv_congr, conv_lt⟩)
 
-def consAppendConverter {xs : Vector α n} {ys : Vector α m} : IndexConverter (Nat.zero_lt_succ _) ys (x ::ᵥ xs.append ys) :=
+def consAppendConverter {xs : Vector α n} {ys : Vector α m} : IndexConverterGtZero ys (x ::ᵥ xs.append ys) :=
   let conv : Fin m → Fin (n + m + 1) := λ i ↦ ⟨i.val + n + 1, by have := i.isLt; linarith⟩
   have conv_congr : ∀ {i}, ys.get i = (x ::ᵥ xs.append ys).get (conv i) := by
     intro i
@@ -123,32 +138,31 @@ def consAppendConverter {xs : Vector α n} {ys : Vector α m} : IndexConverter (
     simp
     exact Vector.get_append_right.symm
   have conv_lt : ∀ ⦃i j⦄, i < j → conv i < conv j := by simp [conv]
-  have conv_gt_zero: ∀ {i}, 0 < conv i := by
+  have conv_gt_zero: ∀ {i}, _ → 0 < conv i := by
     intro i
     simp [conv]
     apply Fin.mk_lt_mk.mpr
     rw [Nat.zero_mod]
     simp
-  ⟨conv, conv_congr, conv_lt, conv_gt_zero⟩
+  .mk conv_gt_zero (toIndexConverter := ⟨conv, conv_congr, conv_lt⟩)
 
-
-def appendConverter {xs : Vector α n} {ys : Vector α m} (h_n : 0 < n) : IndexConverter (by linarith) ys (xs.append ys) :=
+def appendConverter {xs : Vector α n} {ys : Vector α m} (h_n : 0 < n) : IndexConverterGtZero ys (xs.append ys) :=
   let conv : Fin m → Fin (n + m) := λ i ↦ ⟨i.val + n, by have := i.isLt; linarith⟩
   have conv_congr : ∀ {i}, ys.get i = (xs.append ys).get (conv i) := by
     intro i
     exact Vector.get_append_right.symm
   have conv_lt : ∀ ⦃i j⦄, i < j → conv i < conv j := by simp [conv]
-  have conv_gt_zero: ∀ {i}, ⟨0, _⟩ < conv i := by
-    intro i
+  have conv_gt_zero: ∀ {i}, (h_m : 0 < n + m) → ⟨0, h_m⟩ < conv i := by
+    intro i h_m
     simp [conv]
     apply Or.intro_right
     exact h_n
-  ⟨conv, conv_congr, conv_lt, conv_gt_zero⟩
+  .mk conv_gt_zero (toIndexConverter := ⟨conv, conv_congr, conv_lt⟩)
 
 /-- Assume new consumer has index 0. -/
 def convertFifosOutput {inputs outputs : List SimpleDataflow.Ty} {numNodes : Nat} {nodes : SDFNodeList numNodes}
   (h_len : 0 < numNodes) (a : SDFOneOutput α) (newConsumerPort : Member α.toSDF (nodes.get ⟨0, h_len⟩).inputs)
-  (idxConv : IndexConverter h_len a.g.nodes nodes)
+  (idxConv : IndexConverterGtZero a.g.nodes nodes)
   (memConv : {t : SimpleDataflow.Ty} → Member t a.g.inputs → Member t inputs)
   : List (FIFO inputs outputs nodes) :=
   a.g.fifos.attach.map (
@@ -178,23 +192,17 @@ def convertFifosOutput {inputs outputs : List SimpleDataflow.Ty} {numNodes : Nat
           consumer := ⟨0, h_len⟩,
           producerPort := idxConv.conv_congr ▸ f.producerPort,
           consumerPort := h_ty_eq ▸ newConsumerPort,
-          adv := idxConv.conv_gt_zero,
+          adv := idxConv.conv_gt_zero h_len,
         }
         .advancing fifo
       | .advancing f =>
-        let newProducer := idxConv.conv f.producer
-        let newConsumer := idxConv.conv f.consumer
-        have adv : newProducer.val > newConsumer.val := by
-          simp [newProducer, newConsumer]
-          apply idxConv.conv_lt
-          exact f.adv
         let fifo : AdvancingFIFO nodes := {
           t := f.t,
-          producer := newProducer,
-          consumer := newConsumer,
+          producer := idxConv.conv f.producer,
+          consumer := idxConv.conv f.consumer,
           producerPort := idxConv.conv_congr ▸ f.producerPort,
           consumerPort := idxConv.conv_congr ▸ f.consumerPort,
-          adv := adv
+          adv := idxConv.conv_lt f.adv
         }
         .advancing fifo
       | .initialized f =>
@@ -213,7 +221,7 @@ def convertFifosOutput {inputs outputs : List SimpleDataflow.Ty} {numNodes : Nat
 
 theorem convertFifos_no_output {inputs outputs : List SimpleDataflow.Ty} {numNodes : Nat} {nodes : SDFNodeList numNodes}
   {h_len : 0 < numNodes} {a : SDFOneOutput α} {newConsumerPort : Member α.toSDF (nodes.get ⟨0, h_len⟩).inputs}
-  {idxConv : IndexConverter h_len a.g.nodes nodes}
+  {idxConv : IndexConverterGtZero a.g.nodes nodes}
   {memConv : {t : SimpleDataflow.Ty} → Member t a.g.inputs → Member t inputs}
  : (convertFifosOutput h_len a newConsumerPort idxConv memConv).filter
       (@FIFO.isOutput SimpleDataflow.Ty _ _ SimpleDataflow.Ops _ numNodes nodes inputs outputs)
@@ -222,9 +230,59 @@ theorem convertFifos_no_output {inputs outputs : List SimpleDataflow.Ty} {numNod
   intro fifo h_mem
   have h_map := List.mem_map.mp h_mem
   let ⟨⟨fifo', _⟩, ⟨_, h_match⟩⟩ := h_map
-  cases fifo' <;> (simp at h_match; rw [←h_match]; simp)
+  cases fifo' <;> (simp at h_match; rw [←h_match]; simp [FIFO.isOutput])
 
-def mergeTwoGraph (a : SDFOneOutput α) (op : Step.UnaryOp α β) : SDFOneOutput β :=
+def SDFOneInputOneOutput.convertFifosDropInput {numNodes : Nat} {nodes : SDFNodeList numNodes} {inputs : List SimpleDataflow.Ty}
+  (a : SDFOneInputOneOutput α β) (idxConv : IndexConverter a.g.nodes nodes)
+  : List (FIFO inputs [β.toSDF] nodes) :=
+  let filtered := a.g.fifos.filter (λ fifo ↦ (fifo.isInput = false) && (fifo.isOutput = false))
+  filtered.attach.map (
+    λ ⟨fifo, h_mem⟩ ↦
+      have h_not_input : (fifo.isInput = false) ∧ (fifo.isOutput = false) := by
+        have := (List.mem_filter.mp h_mem).right
+        rw [←Bool.decide_and] at this
+        exact of_decide_eq_true this
+      match fifo, h_not_input with
+      | .initialized fifo, _ =>
+        .initialized {
+          t := fifo.t,
+          initialValue := fifo.initialValue,
+          producer := idxConv.conv fifo.producer,
+          consumer := idxConv.conv fifo.consumer,
+          producerPort := idxConv.conv_congr ▸ fifo.producerPort,
+          consumerPort := idxConv.conv_congr ▸ fifo.consumerPort
+        }
+      | .advancing fifo, _ =>
+        .advancing {
+          t := fifo.t,
+          producer := idxConv.conv fifo.producer,
+          consumer := idxConv.conv fifo.consumer,
+          producerPort := idxConv.conv_congr ▸ fifo.producerPort,
+          consumerPort := idxConv.conv_congr ▸ fifo.consumerPort,
+          adv := idxConv.conv_lt fifo.adv
+        }
+  )
+
+theorem SDFOneInputOneOutput.convertFifosDropInput_no_output {numNodes : Nat} {nodes : SDFNodeList numNodes} {inputs : List SimpleDataflow.Ty}
+  {a : SDFOneInputOneOutput α β} {idxConv : IndexConverter a.g.nodes nodes}
+  : (@SDFOneInputOneOutput.convertFifosDropInput α β numNodes nodes inputs a idxConv).filter FIFO.isOutput = [] := by
+  simp only [SDFOneInputOneOutput.convertFifosDropInput]
+  apply List.filter_eq_nil.mpr
+  intro fifo h_mem
+  have := List.mem_map.mp h_mem
+  clear h_mem
+  let ⟨fifo', h_mem⟩ := this
+  clear this
+  rw [←h_mem.right]
+  clear h_mem
+  let ⟨fifo'', h_filter⟩ := fifo'
+  have := (List.mem_filter.mp h_filter).right
+  simp only [Bool.and_eq_true] at this
+  have := this.right
+  have := of_decide_eq_true this
+  split <;> simp [FIFO.isOutput]
+
+def mergeTwoGraphs (a : SDFOneOutput α) (op : Step.UnaryOp α β) : SDFOneOutput β :=
   let inputs := a.g.inputs
   let outputs := [β.toSDF]
   let opGraph := op.compile
@@ -232,8 +290,41 @@ def mergeTwoGraph (a : SDFOneOutput α) (op : Step.UnaryOp α β) : SDFOneOutput
   have h_len_app : 0 < opGraph.g.numNodes + a.g.numNodes := Nat.lt_add_right _ opGraph.nodes_len
   have h_nodes_eq : nodes.get ⟨0, h_len_app⟩ = opGraph.g.nodes.get ⟨0, opGraph.nodes_len⟩ := Vector.get_append_left (xs := opGraph.g.nodes) (ys := a.g.nodes) (i := ⟨0, opGraph.nodes_len⟩)
   let aFifosUpdated : List (FIFO inputs outputs nodes) := convertFifosOutput h_len_app a (h_nodes_eq ▸ opGraph.consumerPort) (appendConverter opGraph.nodes_len) id
-  
-  sorry
+  let opGraphFifosUpdated : List (FIFO inputs outputs nodes) := opGraph.convertFifosDropInput appendIdConverter
+
+  let outIdx := ⟨0, h_len_app⟩
+  have h_producer_eq : opGraph.g.nodes.get opGraph.outFifo.producer = nodes.get outIdx := by
+    rw [opGraph.out_producer]
+    apply Vector.get_append_left.symm
+  let newOutFifo : OutputFIFO outputs nodes := {
+    t := β.toSDF,
+    producer := outIdx,
+    producerPort := opGraph.out_ty_eq ▸ h_producer_eq ▸ opGraph.outFifo.producerPort,
+    consumer := .head
+  }
+
+  let newFifos := .output newOutFifo :: aFifosUpdated ++ opGraphFifosUpdated
+
+  let newGraph : SimpleDataflow.DataflowMachine := {
+    inputs := inputs,
+    outputs := outputs,
+    numNodes := nodes.length,
+    nodes := nodes,
+    fifos := newFifos
+  }
+
+  have one_output : newGraph.fifos.filter FIFO.isOutput = [.output newOutFifo] := by
+    simp [newFifos, FIFO.isOutput]
+    rw [convertFifos_no_output]
+    simp
+    exact opGraph.convertFifosDropInput_no_output
+
+  {
+    g := newGraph,
+    fifo := newOutFifo,
+    one_output := one_output,
+    ty_eq := rfl
+  }
 
 def mergeThreeGraphs (a : SDFOneOutput α) (b : SDFOneOutput β) (op : Step.BinaryOp α β γ) : SDFOneOutput γ :=
   let inputs := a.g.inputs ++ b.g.inputs
@@ -241,8 +332,8 @@ def mergeThreeGraphs (a : SDFOneOutput α) (b : SDFOneOutput β) (op : Step.Bina
   let newNode : SDFNode := ⟨[α.toSDF, β.toSDF], outputs, [], []ₕ, op.compile⟩
   let nodes := newNode ::ᵥ (a.g.nodes.append b.g.nodes)
 
-  let aFifosUpdated : List (FIFO inputs outputs nodes) := convertFifosOutput _ a .head consConverter .append_left
-  let bFifosUpdated : List (FIFO inputs outputs nodes) := convertFifosOutput _ b (.tail .head) consAppendConverter .append_right
+  let aFifosUpdated : List (FIFO inputs outputs nodes) := convertFifosOutput (Nat.zero_lt_succ _) a .head consConverter .append_left
+  let bFifosUpdated : List (FIFO inputs outputs nodes) := convertFifosOutput (Nat.zero_lt_succ _) b (.tail .head) consAppendConverter .append_right
 
   let newOutputFifo : OutputFIFO outputs nodes := {
     t := γ.toSDF,
@@ -260,7 +351,7 @@ def mergeThreeGraphs (a : SDFOneOutput α) (b : SDFOneOutput β) (op : Step.Bina
   }
 
   have one_output : newGraph.fifos.filter FIFO.isOutput = [.output newOutputFifo] := by
-    simp [newFifos]
+    simp [newFifos, FIFO.isOutput]
     apply And.intro convertFifos_no_output convertFifos_no_output
 
   {
@@ -269,6 +360,11 @@ def mergeThreeGraphs (a : SDFOneOutput α) (b : SDFOneOutput β) (op : Step.Bina
     one_output := one_output,
     ty_eq := rfl
   }
+
+def reduceBlock {α β : Step.Prim} {inp : List Step.Ty}
+  (op : Step.BinaryOp α β α) (len : Nat) (init : α.denote) (bs : Step.Prog inp (Step.Ty.stream β))
+  : SDFOneOutput α :=
+  sorry
 
 def Step.Prog.compile {inp : List Step.Ty} {out : Step.Ty} : Step.Prog inp out → out.toSDF
   | .const α =>
@@ -306,13 +402,12 @@ def Step.Prog.compile {inp : List Step.Ty} {out : Step.Ty} : Step.Prog inp out �
     {
       g := graph,
       fifo := outputFifo,
-      one_output := by simp,
+      one_output := by simp [FIFO.isOutput],
       ty_eq := by simp [outputFifo]
     }
   | .zip op as bs =>
     let asg := as.compile
     let bsg := bs.compile
     mergeThreeGraphs asg bsg op
-  | Step.Prog.map op as =>
-    sorry
-  | .reduce op len init bs => sorry
+  | Step.Prog.map op as => mergeTwoGraphs as.compile op
+  | .reduce op len init bs => reduceBlock op len init bs
